pancake/semantics/panItreeSemScript.sml
@@ -344,9 +344,9 @@ Definition h_handle_call_ret_def:
    case calltyp of
      NONE => Ret (SOME (Return retv),empty_locals s')
    | SOME (NONE, _) => Ret (NONE, s' with locals := s.locals)
-   | SOME (SOME rt,_) =>
+   | SOME (SOME (rk,rt),_) =>
        if is_valid_value s.locals rt retv
-       then Ret (NONE,set_var rt retv (s' with locals := s.locals))
+       then Ret (NONE,set_kvar rk rt retv (s' with locals := s.locals))
        else Ret (SOME Error,s')) ∧
   (h_handle_call_ret calltyp s (SOME (Exception eid exn),s') =
    case calltyp of
